Fixed proofs; made unmaintainable theories slightly less so

Semantics/IRStepThms.thy
@@ -12,9 +12,81 @@ transition to the same subsequent configuration. Therefore, our step semantics
 is deterministic.
 \<close>
 
+(*
+definition stepping_nodes :: "(IRNode \<Rightarrow> bool) set" where
+  "stepping_nodes = {
+    is_sequential_node,
+    is_IfNode,
+    is_AbstractEndNode,
+    is_NewInstanceNode,
+    is_LoadFieldNode,
+    is_SignedDivNode,
+    is_SignedRemNode,
+    is_LoadFieldNode,
+    is_StoreFieldNode
+  }"
+
+inductive_cases StepE[elim!]:\<^marker>\<open>tag invisible\<close>
+  "g, p \<turnstile> (nid,m,h) \<rightarrow> next"
+
+lemma stepping_nodes_distinct:
+  assumes "sel \<in> stepping_nodes \<and> sel node"
+  shows "\<forall> oth \<in> stepping_nodes - {sel} . \<not>(oth node)"
+  using assms unfolding stepping_nodes_def sorry
+
+
+proof (induction arbitrary: m h rule: step.induct)
+  case (SequentialNode nid nid')
+  have "is_sequential_node \<in> stepping_nodes" unfolding stepping_nodes_def by simp
+  then have distinct: "\<forall> oth \<in> stepping_nodes - {is_sequential_node} . \<not>(oth (kind g nid))"
+    using stepping_nodes_distinct SequentialNode(1) by auto
+  obtain next' where "g, p \<turnstile> (nid, m, h) \<rightarrow> next'"
+    using SequentialNode.hyps(1) step.SequentialNode
+    by blast
+  then have "next' = (nid', m, h)"
+    apply (induct rule: step.induct) using SequentialNode sorry
+  show ?case apply (rule allI) (*using step.cases*) apply (induction rule: step.induct)
+    using distinct unfolding stepping_nodes_def
+    using is_IfNode_def is_NewInstanceNode_def is_LoadFieldNode_def is_SignedDivNode_def is_SignedRemNode_def
+    is_LoadFieldNode_def is_StoreFieldNode_def 
+    apply (rule stepping_nodes_distinct [where sel = is_sequential_node, where node = "kind g nid"])
+  then show ?case apply (rule stepping_nodes_distinct [where sel = is_sequential_node, where node = "kind g nid"])?
+next
+  case (IfNode nid cond tb fb condE m val nid' h)
+  then show ?case sorry
+next
+  case (EndNodes nid merge i phis inps inpsE m vs m' h)
+  then show ?case sorry
+next
+  case (NewInstanceNode nid f obj nid' h' ref h m' m)
+  then show ?case sorry
+next
+  case (LoadFieldNode nid f obj nid' objE m ref h v m')
+  then show ?case sorry
+next
+  case (SignedDivNode nid x y zero sb nxt xe ye m v1 v2 v m' h)
+  then show ?case sorry
+next
+  case (SignedRemNode nid x y zero sb nxt xe ye m v1 v2 v m' h)
+  then show ?case sorry
+next
+  case (StaticLoadFieldNode nid f nid' h v m' m)
+  then show ?case sorry
+next
+  case (StoreFieldNode nid f newval uu obj nid' newvalE objE m val ref h' h m')
+  then show ?case sorry
+next
+  case (StaticStoreFieldNode nid f newval uv nid' newvalE m val h' h m')
+  then show ?case sorry
+qed
+*)
+
 theorem stepDet:
    "(g, p \<turnstile> (nid,m,h) \<rightarrow> next) \<Longrightarrow>
    (\<forall> next'. ((g, p \<turnstile> (nid,m,h) \<rightarrow> next') \<longrightarrow> next = next'))"
+
+
+
 proof (induction rule: "step.induct")
   case (SequentialNode nid "next" m h)
   have notif: "\<not>(is_IfNode (kind g nid))"
@@ -37,7 +109,7 @@ proof (induction rule: "step.induct")
     by (metis is_IntegerDivRemNode.simps)
   from notif notend notnew notload notstore notdivrem
   show ?case using SequentialNode step.cases
-    by (smt (z3) IRNode.disc(2042) IRNode.disc(920) IRNode.discI(30) Pair_inject is_sequential_node.simps(18) is_sequential_node.simps(41) is_sequential_node.simps(42))
+    by (smt (z3) IRNode.disc(1028) IRNode.disc(2270) IRNode.discI(31) Pair_inject is_sequential_node.simps(18) is_sequential_node.simps(43) is_sequential_node.simps(44))
 next
   case (IfNode nid cond tb fb m val "next" h)
   then have notseq: "\<not>(is_sequential_node (kind g nid))"
@@ -50,7 +122,7 @@ next
     using is_AbstractEndNode.simps
     by (simp add: IfNode.hyps(1))
   from notseq notend notdivrem show ?case using IfNode repDet evalDet IRNode.distinct IRNode.inject(11) Pair_inject step.simps
-    by (smt (z3) IRNode.distinct IRNode.inject(11) Pair_inject step.simps)
+    by (smt (z3) IRNode.distinct IRNode.inject(12) Pair_inject step.simps)
 next
   case (EndNodes nid merge i phis inputs m vs m' h)
   have notseq: "\<not>(is_sequential_node (kind g nid))"
@@ -58,7 +130,7 @@ next
     by (metis is_EndNode.elims(2) is_LoopEndNode_def)
   have notif: "\<not>(is_IfNode (kind g nid))"
     using EndNodes.hyps(1) is_IfNode_def is_AbstractEndNode.elims
-    by (metis IRNode.distinct_disc(989) is_EndNode.simps(12))
+    by (metis IRNode.distinct_disc(1058) is_EndNode.simps(12))
   have notref: "\<not>(is_RefNode (kind g nid))"
     using EndNodes.hyps(1) is_sequential_node.simps
     using IRNode.disc(1899) IRNode.distinct(1473) is_AbstractEndNode.simps is_EndNode.elims(2) is_LoopEndNode_def is_RefNode_def
@@ -66,14 +138,14 @@ next
   have notnew: "\<not>(is_NewInstanceNode (kind g nid))"
     using EndNodes.hyps(1) is_AbstractEndNode.simps
     using IRNode.distinct_disc(1442) is_EndNode.simps(29) is_NewInstanceNode_def
-    by (metis IRNode.distinct_disc(1710) is_EndNode.simps(31))
+    by (metis IRNode.distinct_disc(1901) is_EndNode.simps(32))
   have notload: "\<not>(is_LoadFieldNode (kind g nid))"
     using EndNodes.hyps(1) is_AbstractEndNode.simps
-    by (metis IRNode.distinct_disc(1526) is_EndNode.simps(20) is_LoadFieldNode_def)
+    using is_LoadFieldNode_def
+    by (metis IRNode.distinct_disc(1706) is_EndNode.simps(21))
   have notstore: "\<not>(is_StoreFieldNode (kind g nid))"
-    using EndNodes.hyps(1) is_AbstractEndNode.simps
-    using IRNode.distinct_disc(1504) is_EndNode.simps(39) is_StoreFieldNode_def 
-    by fastforce
+    using EndNodes.hyps(1) is_AbstractEndNode.simps is_StoreFieldNode_def
+    by (metis IRNode.distinct_disc(1926) is_EndNode.simps(44))
   have notdivrem: "\<not>(is_IntegerDivRemNode (kind g nid))"
     using EndNodes.hyps(1) is_AbstractEndNode.simps is_SignedDivNode_def is_SignedRemNode_def
     using IRNode.distinct_disc(1498) IRNode.distinct_disc(1500) is_IntegerDivRemNode.simps is_EndNode.simps(36) is_EndNode.simps(37) 
@@ -106,7 +178,7 @@ next
     by (simp add: NewInstanceNode.hyps(1))
   from notseq notend notif notref notload notstore notdivrem
   show ?case using NewInstanceNode step.cases
-    by (smt (verit) IRNode.distinct(2085) IRNode.distinct(2087) IRNode.inject(30) Pair_inject is_IfNode_def is_LoadFieldNode_def is_StoreFieldNode_def)
+    by (smt (z3) IRNode.disc(1028) IRNode.disc(2270) IRNode.discI(11) IRNode.distinct(2311) IRNode.distinct(2313) IRNode.inject(31) Pair_inject)
 next
   case (LoadFieldNode nid f obj nxt m ref h v m')
   then have notseq: "\<not>(is_sequential_node (kind g nid))"
@@ -120,7 +192,7 @@ next
     by (simp add: LoadFieldNode.hyps(1))
   from notseq notend notdivrem
   show ?case using LoadFieldNode step.cases repDet evalDet
-    by (smt (verit) IRNode.distinct(1541) IRNode.distinct(1557) IRNode.distinct(1559) IRNode.distinct(1563) IRNode.distinct(983) IRNode.inject(19) Pair_inject Value.inject(3) option.discI option.inject)
+    by (smt (z3) IRNode.distinct(1051) IRNode.distinct(1721) IRNode.distinct(1739) IRNode.distinct(1741) IRNode.distinct(1745) IRNode.inject(20) Pair_inject Value.inject(3) option.distinct(1) option.inject)
 next
   case (StaticLoadFieldNode nid f nxt h v m' m)
   then have notseq: "\<not>(is_sequential_node (kind g nid))"
@@ -133,7 +205,7 @@ next
     by (simp add: StaticLoadFieldNode.hyps(1))
   from notseq notend notdivrem
   show ?case using StaticLoadFieldNode step.cases
-    by (smt (z3) IRNode.distinct(1541) IRNode.distinct(1557) IRNode.distinct(1559) IRNode.distinct(1563) IRNode.distinct(983) IRNode.inject(19) Pair_inject option.distinct(1))
+    by (smt (z3) IRNode.distinct(1051) IRNode.distinct(1721) IRNode.distinct(1739) IRNode.distinct(1741) IRNode.distinct(1745) IRNode.inject(20) Pair_inject option.distinct(1))
 next
   case (StoreFieldNode nid f newval uu obj nxt m val ref h' h m')
   then have notseq: "\<not>(is_sequential_node (kind g nid))"
@@ -146,7 +218,7 @@ next
     by (simp add: StoreFieldNode.hyps(1))
   from notseq notend notdivrem
   show ?case using StoreFieldNode step.cases repDet evalDet
-    by (smt (verit) IRNode.distinct(1027) IRNode.distinct(1563) IRNode.distinct(2091) IRNode.distinct(2323) IRNode.distinct(2343) IRNode.inject(41) Pair_inject Value.inject(3) option.discI option.inject)
+    by (smt (z3) IRNode.distinct(1097) IRNode.distinct(1745) IRNode.distinct(2317) IRNode.distinct(2605) IRNode.distinct(2627) IRNode.inject(43) Pair_inject Value.inject(3) option.distinct(1) option.inject)
 next
   case (StaticStoreFieldNode nid f newval uv nxt m val h' h m')
   then have notseq: "\<not>(is_sequential_node (kind g nid))"
@@ -159,7 +231,7 @@ next
     by (simp add: StaticStoreFieldNode.hyps(1))
   from notseq notend notdivrem
   show ?case using StoreFieldNode step.cases repDet evalDet
-    by (smt (z3) IRNode.distinct(1027) IRNode.distinct(1563) IRNode.distinct(2091) IRNode.distinct(2323) IRNode.distinct(2343) IRNode.inject(41) Pair_inject StaticStoreFieldNode.hyps(1) StaticStoreFieldNode.hyps(2) StaticStoreFieldNode.hyps(3) StaticStoreFieldNode.hyps(4) StaticStoreFieldNode.hyps(5) option.distinct(1))
+    by (smt (z3) IRNode.distinct(1097) IRNode.distinct(1745) IRNode.distinct(2317) IRNode.distinct(2605) IRNode.distinct(2627) IRNode.inject(43) Pair_inject StaticStoreFieldNode.hyps(1) StaticStoreFieldNode.hyps(2) StaticStoreFieldNode.hyps(3) StaticStoreFieldNode.hyps(4) StaticStoreFieldNode.hyps(5) option.distinct(1))
 next
   case (SignedDivNode nid x y zero sb nxt m v1 v2 v m' h)
   then have notseq: "\<not>(is_sequential_node (kind g nid))"
@@ -170,7 +242,7 @@ next
     by (simp add: SignedDivNode.hyps(1))
   from notseq notend
   show ?case using SignedDivNode step.cases repDet evalDet
-    by (smt (z3) IRNode.distinct(1021) IRNode.distinct(1557) IRNode.distinct(2085) IRNode.distinct(2319) IRNode.distinct(2323) IRNode.inject(38) Pair_inject)
+    by (smt (z3) IRNode.distinct(1091) IRNode.distinct(1739) IRNode.distinct(2311) IRNode.distinct(2601) IRNode.distinct(2605) IRNode.inject(40) Pair_inject)
 next
   case (SignedRemNode nid x y zero sb nxt m v1 v2 v m' h)
   then have notseq: "\<not>(is_sequential_node (kind g nid))"
@@ -181,7 +253,7 @@ next
     by (simp add: SignedRemNode.hyps(1))
   from notseq notend
   show ?case using SignedRemNode step.cases repDet evalDet
-    by (smt (z3) IRNode.distinct(1023) IRNode.distinct(1559) IRNode.distinct(2087) IRNode.distinct(2319) IRNode.distinct(2343) IRNode.inject(39) Pair_inject)
+    by (smt (z3) IRNode.distinct(1093) IRNode.distinct(1741) IRNode.distinct(2313) IRNode.distinct(2601) IRNode.distinct(2627) IRNode.inject(41) Pair_inject)
 qed
 
 lemma stepRefNode:
@@ -214,11 +286,11 @@ lemma step_in_ids:
   using assms apply (induct "(nid, m, h)" "(nid', m', h')" rule: step.induct)
   using is_sequential_node.simps(45) not_in_g 
   apply simp
-  apply (metis is_sequential_node.simps(50))
+  apply (metis is_sequential_node.simps(53))
   using ids_some
-  using IRNode.distinct(1041) apply presburger
+  using IRNode.distinct(1113) apply presburger
   using EndNodes(1) is_AbstractEndNode.simps is_EndNode.simps(45) ids_some
-  apply (metis IRNode.disc(1099) is_EndNode.simps(49))
+  apply (metis IRNode.disc(1218) is_EndNode.simps(52))
   by simp+
 
 end
