Semantics/IRTreeEvalThms.thy
@@ -3,6 +3,7 @@ section \<open>Data-flow Expression-Tree Theorems\<close>
 theory IRTreeEvalThms
   imports
     TreeToGraph
+    "HOL-Eisbach.Eisbach"
 begin
 
 
@@ -13,148 +14,150 @@ text \<open>First, we prove some extra rules that relate each
   These are very helpful for proving that 'rep' is deterministic.
 \<close>
 
-lemma rep_constant: 
+named_theorems rep
+
+lemma rep_constant [rep]: 
   "g \<turnstile> n \<simeq> e \<Longrightarrow> 
    kind g n = ConstantNode c \<Longrightarrow> 
    e = ConstantExpr c"
   by (induction rule: rep.induct; auto)
   
-lemma rep_parameter: 
+lemma rep_parameter [rep]: 
   "g \<turnstile> n \<simeq> e \<Longrightarrow> 
    kind g n = ParameterNode i \<Longrightarrow>
    (\<exists>s. e = ParameterExpr i s)"
   by (induction rule: rep.induct; auto)
 
-lemma rep_conditional:
+lemma rep_conditional [rep]:
   "g \<turnstile> n \<simeq> e \<Longrightarrow>
    kind g n = ConditionalNode c t f \<Longrightarrow>
    (\<exists> ce te fe. e = ConditionalExpr ce te fe)"
   by (induction rule: rep.induct; auto)
 
-lemma rep_abs:
+lemma rep_abs [rep]:
   "g \<turnstile> n \<simeq> e \<Longrightarrow>
    kind g n = AbsNode x \<Longrightarrow>
    (\<exists>xe. e = UnaryExpr UnaryAbs xe)"
   by (induction rule: rep.induct; auto)
 
-lemma rep_not:
+lemma rep_not [rep]:
   "g \<turnstile> n \<simeq> e \<Longrightarrow>
    kind g n = NotNode x \<Longrightarrow>
    (\<exists>xe. e = UnaryExpr UnaryNot xe)"
   by (induction rule: rep.induct; auto)
 
-lemma rep_negate:
+lemma rep_negate [rep]:
   "g \<turnstile> n \<simeq> e \<Longrightarrow>
    kind g n = NegateNode x \<Longrightarrow>
    (\<exists>xe. e = UnaryExpr UnaryNeg xe)"
   by (induction rule: rep.induct; auto)
 
-lemma rep_logicnegation:
+lemma rep_logicnegation [rep]:
   "g \<turnstile> n \<simeq> e \<Longrightarrow>
    kind g n = LogicNegationNode x \<Longrightarrow>
    (\<exists>xe. e = UnaryExpr UnaryLogicNegation xe)"
   by (induction rule: rep.induct; auto)
 
-lemma rep_add:
+lemma rep_add [rep]:
   "g \<turnstile> n \<simeq> e \<Longrightarrow>
    kind g n = AddNode x y \<Longrightarrow>
    (\<exists>xe ye. e = BinaryExpr BinAdd xe ye)"
   by (induction rule: rep.induct; auto)
 
-lemma rep_sub:
+lemma rep_sub [rep]:
   "g \<turnstile> n \<simeq> e \<Longrightarrow>
    kind g n = SubNode x y \<Longrightarrow>
    (\<exists>xe ye. e = BinaryExpr BinSub xe ye)"
   by (induction rule: rep.induct; auto)
 
-lemma rep_mul:
+lemma rep_mul [rep]:
   "g \<turnstile> n \<simeq> e \<Longrightarrow>
    kind g n = MulNode x y \<Longrightarrow>
    (\<exists>xe ye. e = BinaryExpr BinMul xe ye)"
   by (induction rule: rep.induct; auto)
 
-lemma rep_and:
+lemma rep_and [rep]:
   "g \<turnstile> n \<simeq> e \<Longrightarrow>
    kind g n = AndNode x y \<Longrightarrow>
    (\<exists>xe ye. e = BinaryExpr BinAnd xe ye)"
   by (induction rule: rep.induct; auto)
 
-lemma rep_or:
+lemma rep_or [rep]:
   "g \<turnstile> n \<simeq> e \<Longrightarrow>
    kind g n = OrNode x y \<Longrightarrow>
    (\<exists>xe ye. e = BinaryExpr BinOr xe ye)"
   by (induction rule: rep.induct; auto)
 
-lemma rep_xor:
+lemma rep_xor [rep]:
   "g \<turnstile> n \<simeq> e \<Longrightarrow>
    kind g n = XorNode x y \<Longrightarrow>
    (\<exists>xe ye. e = BinaryExpr BinXor xe ye)"
   by (induction rule: rep.induct; auto)
 
-lemma rep_integer_below:
+lemma rep_integer_below [rep]:
   "g \<turnstile> n \<simeq> e \<Longrightarrow>
    kind g n = IntegerBelowNode x y \<Longrightarrow>
    (\<exists>xe ye. e = BinaryExpr BinIntegerBelow xe ye)"
   by (induction rule: rep.induct; auto)
 
-lemma rep_integer_equals:
+lemma rep_integer_equals [rep]:
   "g \<turnstile> n \<simeq> e \<Longrightarrow>
    kind g n = IntegerEqualsNode x y \<Longrightarrow>
    (\<exists>xe ye. e = BinaryExpr BinIntegerEquals xe ye)"
   by (induction rule: rep.induct; auto)
 
-lemma rep_integer_less_than:
+lemma rep_integer_less_than [rep]:
   "g \<turnstile> n \<simeq> e \<Longrightarrow>
    kind g n = IntegerLessThanNode x y \<Longrightarrow>
    (\<exists>xe ye. e = BinaryExpr BinIntegerLessThan xe ye)"
   by (induction rule: rep.induct; auto)
 
-lemma rep_narrow:
+lemma rep_narrow [rep]:
   "g \<turnstile> n \<simeq> e \<Longrightarrow>
    kind g n = NarrowNode ib rb x \<Longrightarrow>
    (\<exists>x. e = UnaryExpr (UnaryNarrow ib rb) x)"
   by (induction rule: rep.induct; auto)
  
-lemma rep_sign_extend:
+lemma rep_sign_extend [rep]:
   "g \<turnstile> n \<simeq> e \<Longrightarrow>
    kind g n = SignExtendNode ib rb x \<Longrightarrow>
    (\<exists>x. e = UnaryExpr (UnarySignExtend ib rb) x)"
   by (induction rule: rep.induct; auto)
 
-lemma rep_zero_extend:
+lemma rep_zero_extend [rep]:
   "g \<turnstile> n \<simeq> e \<Longrightarrow>
    kind g n = ZeroExtendNode ib rb x \<Longrightarrow>
    (\<exists>x. e = UnaryExpr (UnaryZeroExtend ib rb) x)"
   by (induction rule: rep.induct; auto)
 
-lemma rep_load_field:
+lemma rep_load_field [rep]:
   "g \<turnstile> n \<simeq> e \<Longrightarrow>
    is_preevaluated (kind g n) \<Longrightarrow>
    (\<exists>s. e = LeafExpr n s)"
   by (induction rule: rep.induct; auto)
 
-lemmas reps =
-  rep_constant
-  rep_parameter
-  rep_conditional
-  rep_abs
-  rep_not
-  rep_negate
-  rep_logicnegation
-  rep_add
-  rep_sub
-  rep_mul
-  rep_and
-  rep_or
-  rep_xor
-  rep_integer_below
-  rep_integer_equals
-  rep_integer_less_than
-  rep_narrow
-  rep_sign_extend
-  rep_zero_extend
-  rep_load_field
 
+method solve_det uses node =
+  (match node in "kind _ _ = node _" for node \<Rightarrow> 
+    \<open>match rep in r: "_ \<Longrightarrow> _ = node _ \<Longrightarrow> _" \<Rightarrow> 
+      \<open>match IRNode.inject in i: "(node _ = node _) = _" \<Rightarrow>
+        \<open>match RepE in e: "_ \<Longrightarrow> (\<And>x. _ = node x \<Longrightarrow> _) \<Longrightarrow> _" \<Rightarrow>
+          \<open>metis i e r\<close>\<close>\<close>\<close> |
+   match node in "kind _ _ = node _ _" for node \<Rightarrow> 
+    \<open>match rep in r: "_ \<Longrightarrow> _ = node _ _ \<Longrightarrow> _" \<Rightarrow> 
+      \<open>match IRNode.inject in i: "(node _ _ = node _ _) = _" \<Rightarrow>
+        \<open>match RepE in e: "_ \<Longrightarrow> (\<And>x y. _ = node x y \<Longrightarrow> _) \<Longrightarrow> _" \<Rightarrow>
+          \<open>metis i e r\<close>\<close>\<close>\<close> |
+   match node in "kind _ _ = node _ _ _" for node \<Rightarrow> 
+    \<open>match rep in r: "_ \<Longrightarrow> _ = node _ _ _ \<Longrightarrow> _" \<Rightarrow> 
+      \<open>match IRNode.inject in i: "(node _ _ _ = node _ _ _) = _" \<Rightarrow>
+        \<open>match RepE in e: "_ \<Longrightarrow> (\<And>x y z. _ = node x y z \<Longrightarrow> _) \<Longrightarrow> _" \<Rightarrow>
+          \<open>metis i e r\<close>\<close>\<close>\<close> |
+  match node in "kind _ _ = node _ _ _" for node \<Rightarrow> 
+    \<open>match rep in r: "_ \<Longrightarrow> _ = node _ _ _ \<Longrightarrow> _" \<Rightarrow> 
+      \<open>match IRNode.inject in i: "(node _ _ _ = node _ _ _) = _" \<Rightarrow>
+        \<open>match RepE in e: "_ \<Longrightarrow> (\<And>x. _ = node _ _ x \<Longrightarrow> _) \<Longrightarrow> _" \<Rightarrow>
+          \<open>metis i e r\<close>\<close>\<close>\<close>)
 
 text \<open>Now we can prove that 'rep' and 'eval', and their list versions, are deterministic.
 \<close>
@@ -169,66 +172,67 @@ next
 next
   case (ConditionalNode n c t f ce te fe)
   then show ?case 
-    by (metis rep_conditional ConditionalNodeE IRNode.inject(6)) 
+    by (solve_det node: ConditionalNode)
 next
   case (AbsNode n x xe)
   then show ?case 
-    by (metis rep_abs AbsNodeE IRNode.inject(1))
+    by (solve_det node: AbsNode)
 next
   case (NotNode n x xe)
   then show ?case
-    by (metis IRNode.inject(32) NotNodeE rep_not)
+    by (solve_det node: NotNode)
 next
   case (NegateNode n x xe)
   then show ?case
-    by (metis  IRNode.inject(29) NegateNodeE rep_negate)
+    by (solve_det node: NegateNode)
 next
   case (LogicNegationNode n x xe)
   then show ?case
-    by (metis IRNode.inject(21) LogicNegationNodeE rep_logicnegation)
+    by (solve_det node: LogicNegationNode)
 next
   case (AddNode n x y xe ye)
   then show ?case
-    by (metis AddNodeE IRNode.inject(2) rep_add) 
+    by (solve_det node: AddNode)
 next
   case (MulNode n x y xe ye)
   then show ?case
-    by (metis IRNode.inject(27) MulNodeE rep_mul)
+    by (solve_det node: MulNode)
 next
   case (SubNode n x y xe ye)
   then show ?case
-    by (metis IRNode.inject(44) SubNodeE rep_sub)
+    by (solve_det node: SubNode)
 next
   case (AndNode n x y xe ye)
   then show ?case
-    by (metis AndNodeE IRNode.inject(3) rep_and)
+    by (solve_det node: AndNode)
 next
   case (OrNode n x y xe ye)
   then show ?case
-  by (metis IRNode.inject(33) OrNodeE rep_or)
+    by (solve_det node: OrNode)
 next
   case (XorNode n x y xe ye)
   then show ?case
-    by (metis IRNode.inject(49) XorNodeE rep_xor)
+    by (solve_det node: XorNode)
 next
   case (IntegerBelowNode n x y xe ye)
   then show ?case
-    by (metis IRNode.inject(12) IntegerBelowNodeE rep_integer_below)
+    by (solve_det node: IntegerBelowNode)
 next
   case (IntegerEqualsNode n x y xe ye)
   then show ?case
-    by (metis IRNode.inject(13) IntegerEqualsNodeE rep_integer_equals)
+    by (solve_det node: IntegerEqualsNode)
 next
   case (IntegerLessThanNode n x y xe ye)
   then show ?case
-    by (metis IRNode.inject(14) IntegerLessThanNodeE rep_integer_less_than)
+    by (solve_det node: IntegerLessThanNode)
 next
   case (NarrowNode n x xe)
-  then show ?case
+  then show ?case   
     by (metis IRNode.inject(28) NarrowNodeE rep_narrow)
 next
   case (SignExtendNode n x xe)
   then show ?case
+    using SignExtendNodeE rep_sign_extend IRNode.inject(39)
     by (metis IRNode.inject(39) SignExtendNodeE rep_sign_extend)
 next
   case (ZeroExtendNode n x xe)
